Give up exporting deduction for now. What should be done next is: reformulate deduction & and use deduction for help in axiomatization proof instead of the other direction.

LogicGenerator/demo/implementation_4.v
@@ -3,10 +3,11 @@ Require Import ZArith.
 Module NaiveLang.
   Definition expr := (nat -> option Z) -> Prop.
   Definition context := expr -> Prop.
+  Definition impp (e1 e2 : expr) : expr := fun st => e1 st -> e2 st.
   Definition andp (e1 e2 : expr) : expr := fun st => e1 st /\ e2 st.
   Definition orp  (e1 e2 : expr) : expr := fun st => e1 st \/ e2 st.
   Definition falsep : expr := fun st => False.
-  Definition truep : expr := fun st => True.
+  Definition coq_prop (P: Prop): expr := fun _ => P.
 
   Definition join : (nat -> option Z) -> (nat -> option Z) -> (nat -> option Z) -> Prop :=
     fun x y z =>
@@ -18,29 +19,62 @@ Module NaiveLang.
     exists st1 st2, join st1 st2 st /\ e1 st1 /\ e2 st2.
   Definition emp : expr := fun st =>
     forall p, st p = None.
-  Definition derivable1 (e1 e2 : expr) : Prop := forall st, e1 st -> e2 st.
+  Definition corable (e: expr): Prop := forall s1 s2, e s1 <-> e s2.
+  
+  Definition provable (e : expr) : Prop := forall st, e st.
 End NaiveLang.
 
 Require Import interface_4.
 
 Module NaiveRule.
   Include DerivedNames (NaiveLang).
-  Axiom falsep_sepcon_left : (forall x : expr, derivable1 (sepcon falsep x) falsep) .
-  Axiom orp_sepcon_left : (forall x y z : expr, derivable1 (sepcon (orp x y) z) (orp (sepcon x z) (sepcon y z))) .
-  Axiom sepcon_emp_left : (forall x : expr, derivable1 (sepcon x emp) x) .
-  Axiom sepcon_emp_right : (forall x : expr, derivable1 x (sepcon x emp)) .
-  Axiom derivable1_sepcon_comm : (forall x y : expr, derivable1 (sepcon x y) (sepcon y x)) .
-  Axiom derivable1_sepcon_assoc1 : (forall x y z : expr, derivable1 (sepcon x (sepcon y z)) (sepcon (sepcon x y) z)) .
-  Axiom derivable1_sepcon_mono : (forall x1 x2 y1 y2 : expr, derivable1 x1 x2 -> derivable1 y1 y2 -> derivable1 (sepcon x1 y1) (sepcon x2 y2)) .
-  Axiom derivable1_truep_intros : (forall x : expr, derivable1 x truep) .
-  Axiom derivable1_falsep_elim : (forall x : expr, derivable1 falsep x) .
-  Axiom derivable1_orp_intros1 : (forall x y : expr, derivable1 x (orp x y)) .
-  Axiom derivable1_orp_intros2 : (forall x y : expr, derivable1 y (orp x y)) .
-  Axiom derivable1_orp_elim : (forall x y z : expr, derivable1 x z -> derivable1 y z -> derivable1 (orp x y) z) .
-  Axiom derivable1_andp_intros : (forall x y z : expr, derivable1 x y -> derivable1 x z -> derivable1 x (andp y z)) .
-  Axiom derivable1_andp_elim1 : (forall x y : expr, derivable1 (andp x y) x) .
-  Axiom derivable1_andp_elim2 : (forall x y : expr, derivable1 (andp x y) y) .
+  Lemma modus_ponens :
+    forall x y : expr, provable (impp x y) -> provable x -> provable y.
+  Proof. unfold provable, impp. auto. Qed.
 
+  Lemma axiom1 : forall x y : expr, provable (impp x (impp y x)).
+  Proof. unfold provable, impp. auto. Qed.
+
+  Lemma axiom2 : forall x y z : expr,
+      provable (impp (impp x (impp y z)) (impp (impp x y) (impp x z))).
+  Proof. unfold provable, impp. auto. Qed.
+
+  Lemma andp_intros :
+    forall x y : expr, provable (impp x (impp y (andp x y))).
+  Proof. unfold provable, impp, andp. auto. Qed.
+
+  Lemma andp_elim1 : forall x y : expr, provable (impp (andp x y) x).
+  Proof. unfold provable, impp, andp. tauto. Qed.
+
+  Lemma andp_elim2 : forall x y : expr, provable (impp (andp x y) y).
+  Proof. unfold provable, impp, andp. tauto. Qed.
+
+  Lemma orp_intros1 : forall x y : expr, provable (impp x (orp x y)).
+  Proof. unfold provable, impp, orp. auto. Qed.
+
+  Lemma orp_intros2 : forall x y : expr, provable (impp y (orp x y)).
+  Proof. unfold provable, impp, orp. auto. Qed.
+
+  Lemma orp_elim : forall x y z : expr,
+      provable (impp (impp x z) (impp (impp y z) (impp (orp x y) z))).
+  Proof. unfold provable, impp, orp. tauto. Qed.
+
+  Lemma falsep_elim : forall x : expr, provable (impp falsep x).
+  Proof. unfold provable, impp, falsep. destruct 1. Qed.
+
+  Lemma peirce_law : forall x y: expr, provable (impp (impp (impp x y) x) x).
+  Proof. unfold provable, impp. intros; tauto. Qed.
+
+  Axiom sepcon_comm: forall x y, provable (iffp (sepcon x y) (sepcon y x)).
+  Axiom sepcon_assoc: forall x y z,
+      provable (iffp (sepcon x (sepcon y z)) (sepcon (sepcon x y) z)).
+  Axiom sepcon_mono : (forall x1 x2 y1 y2 : expr, provable (impp x1 x2) -> provable (impp y1 y2) -> provable (impp (sepcon x1 y1) (sepcon x2 y2))) .
+  Axiom sepcon_emp : (forall x : expr, provable (iffp (sepcon x emp) x)) .
+  Axiom falsep_sepcon_left : (forall x : expr, provable (impp (sepcon falsep x) falsep)) .
+  Axiom orp_sepcon_left : (forall x y z : expr, provable (impp (sepcon (orp x y) z) (orp (sepcon x z) (sepcon y z)))) .
+  Axiom corable_coq_prop : (forall P : Prop, corable (coq_prop P)) .
+  Axiom corable_preserved' : (forall x y : expr, provable (iffp x y) -> corable x -> corable y) .
+  Axiom corable_andp_sepcon1 : (forall x y z : expr, corable x -> provable (iffp (sepcon (andp x y) z) (andp x (sepcon y z)))) .
 End NaiveRule.
 
 Module T := LogicTheorem NaiveLang NaiveRule.
