LogicGenerator/demo/configuration_4.v
@@ -5,30 +5,42 @@ Require Import Logic.LogicGenerator.ConfigLang.
 Import ListNotations.
 
 Definition how_connectives :=
-  [primitive_connective andp
+  [primitive_connective impp
+  ;primitive_connective andp
   ;primitive_connective orp
   ;primitive_connective falsep
-  ;primitive_connective truep
+  ;primitive_connective coq_prop
   ;primitive_connective sepcon
   ;primitive_connective emp
+  ;FROM_andp_impp_TO_iffp
+  ;FROM_falsep_impp_TO_negp
+  ;FROM_falsep_impp_TO_truep
+  ;FROM_impp_TO_multi_imp
+  ;FROM_empty_set_TO_empty_context
   ;FROM_andp_TO_iter_andp
   ;FROM_sepcon_TO_iter_sepcon
   ].
 
 Definition how_judgements :=
-  [primitive_judgement derivable1
+  [primitive_judgement provable
+  ;primitive_judgement corable
+  ;FROM_provable_TO_derivable
   ].
 
 Definition transparent_names :=
   [expr:parameter].
 
 Definition primitive_rule_classes :=
-  [ derivitive1_OF_andp
-  ; derivitive1_OF_orp
-  ; derivitive1_OF_falsep
-  ; derivitive1_OF_truep
-  ; derivitive1_OF_sepcon
-  ; derivitive1_OF_emp
-  ; derivitive1_OF_sepcon_orp_rule
-  ; derivitive1_OF_sepcon_falsep_rule
+  [ provability_OF_impp
+  ; provability_OF_andp
+  ; provability_OF_orp
+  ; provability_OF_falsep
+  ; provability_OF_classical_logic
+  ; provability_OF_sepcon_rule_AS_weak_iffp
+  ; provability_OF_sepcon_rule_AS_mono
+  ; provability_OF_sepcon_orp_rule
+  ; provability_OF_sepcon_falsep_rule
+  ; provability_OF_emp_rule_AS_iffp
+  ; corability_OF_basic_setting
+  ; corability_OF_coq_prop
   ].
