LogicGenerator/demo/configuration_4_ideal.v
@@ -1,0 +1,34 @@
+Require Import Coq.Lists.List.
+Require Import Logic.LogicGenerator.Utils.
+Require Import Logic.LogicGenerator.ConfigLang.
+
+Import ListNotations.
+
+Definition how_connectives :=
+  [primitive_connective andp
+  ;primitive_connective orp
+  ;primitive_connective falsep
+  ;primitive_connective truep
+  ;primitive_connective sepcon
+  ;primitive_connective emp
+  ;FROM_andp_TO_iter_andp
+  ;FROM_sepcon_TO_iter_sepcon
+  ].
+
+Definition how_judgements :=
+  [primitive_judgement derivable1
+  ].
+
+Definition transparent_names :=
+  [expr:parameter].
+
+Definition primitive_rule_classes :=
+  [ derivitive1_OF_andp
+  ; derivitive1_OF_orp
+  ; derivitive1_OF_falsep
+  ; derivitive1_OF_truep
+  ; derivitive1_OF_sepcon
+  ; derivitive1_OF_emp
+  ; derivitive1_OF_sepcon_orp_rule
+  ; derivitive1_OF_sepcon_falsep_rule
+  ].
